theories/program_logic/delayfreewp.v
@@ -1,0 +1,43 @@
+From stdpp Require Import base gmap.
+From iris.algebra Require Import auth gmap excl.
+From iris.proofmode Require Import base tactics classes.
+From iris.base_logic.lib Require Export fancy_updates.
+From shiris.program_logic Require Import delayfree.
+Set Default Proof Using "Type".
+
+(* Curry the value R so it can be changed by the dependent pattern match on c *)
+Definition foo {V R} (c: envE V R) (σ σ': gmap loc V): R -> Prop.
+refine (match c with
+        |GetE l  => λ v, σ !! l = Some v /\ σ' = σ 
+        |PutE l v' => λ _, is_Some (σ !! l) /\ σ' = <[l := v']> σ
+        |AllocE v' => λ _, True
+        |FreeE l => λ _, True 
+        end
+).
+Defined.
+
+Definition wp_pre {Σ} {V} (SI: gmap loc V -> iProp Σ)
+     (go: discrete_funO (λ R, expr V R -d> (R -d> iPropO Σ) -d> iPropO Σ)):
+     discrete_funO (λ R, expr V R -d> (R -d> iPropO Σ) -d> iPropO Σ).
+refine(λ R e Φ,
+        match e with
+        |Answer x => Φ x 
+        |Think e' => ▷ go R e' Φ
+        |Fork e' k => ▷ (go R k Φ ∗ go unit e' (λ _, True))
+        |Vis c k => ∀σ, SI σ ==∗ ∃σ' v, ⌜foo c σ σ' v⌝ ∗ SI σ' ∗ ▷ (go R (k v)) Φ
+        end
+)%I.
+Defined.
+
+Instance wp_pre_contractive {Σ A SI}: Contractive (@wp_pre Σ A SI).
+Proof.
+  rewrite /wp_pre => n wp wp' Hwp R e1 Φ.
+  repeat (f_contractive || f_equiv); apply Hwp.
+Qed.
+
+Definition wp' {Σ} {V} (SI: gmap nat V -> iProp Σ)
+              : ∀R, expr V R -> (R -> iProp Σ) ->iProp Σ :=
+    fixpoint (wp_pre SI ).
+
+Definition wp {Σ} {V R} (SI: gmap nat V -> iProp Σ) (e: expr V R) (Φ: R -> iProp Σ): iProp Σ := 
+    wp' SI R e Φ.
